Prove generalized bitmap allocator spec, good for any [addr]-indexed separation logic memory
The specification for the generalized allocator, [BALLOC.alloc_gen_ok] and
[BALLOC.free_gen_ok], says that there's a predicate associated with every
allocator state.  Their postconditions say that, when [BALLOC.free_gen] is
called, this predicate grows by one block (the freed block).  Conversely,
when [BALLOC.alloc_gen] is called, the predicate shrinks by one block
(the allocated block).

Instantiating this generalized bitmap allocator for allocating disk
blocks is easy: this predicate is simply [sep_star]'ed into the same
memory that's storing the disk blocks.  Indeed, this patch also builds
the regular block allocator in this style, with surprisingly short proofs.

Instantiating the generalized allocator for inodes should be "just"
a matter of [sep_star]'ing this predicate into the inode memory instead
of the disk block memory.

This brings up an interesting point: it seems like the inode allocator
should be part of the directory layer -- not the inode layer!  From this
generalized allocator point of view, allocation is a question of who
owns the inode: either the allocator (through this shrinking/growing
predicate), or something else (through some other predicate that should
probably look like BFile's [file_match] and [data_match]), and this
something else is probably a directory entry.

It seems like we should write a predicate saying that each filename maps
to a unique inum in the inode memory.  Supporting hard links seems hard
because then multiple directory entries own a single inode, and that's
tricky to represent in separation logic.

src/Balloc.v
@@ -197,14 +197,95 @@ Module BALLOC.
   Hint Extern 1 ({{_}} progseq (alloc' _ _ _) _) => apply alloc'_ok : prog.
 
   (* Different names just so that we can state another theorem about them *)
-  Definition alloc := alloc'.
-  Definition free := free'.
+  Definition alloc_gen := alloc'.
+  Definition free_gen := free'.
 
-  Definition rep xp (freeblocks : list addr) :=
+  Definition rep_gen V xp (freeblocks : list addr) (genpred : @pred _ (@weq addrlen) V) :=
     (exists bmap,
      rep' xp bmap *
      [[ forall a, In a freeblocks <-> bmap a = Avail ]] *
-     listpred (fun a => a |->?) freeblocks)%pred.
+     [[ genpred = listpred (fun a => a |->?) freeblocks ]])%pred.
+
+  Theorem alloc_gen_ok : forall V lxp xp mscs,
+    {< Fm mbase m freeblocks genpred,
+    PRE            MEMLOG.rep lxp (ActiveTxn mbase m) mscs *
+                   [[ (Fm * @rep_gen V xp freeblocks genpred)%pred (list2mem m) ]]
+    POST:(mscs',r) [[ r = None ]] * MEMLOG.rep lxp (ActiveTxn mbase m) mscs' \/
+                   exists bn m' freeblocks' genpred', [[ r = Some bn ]] *
+                   MEMLOG.rep lxp (ActiveTxn mbase m') mscs' *
+                   [[ (Fm * @rep_gen V xp freeblocks' genpred')%pred (list2mem m') ]] *
+                   [[ genpred =p=> genpred' * bn |->? ]] *
+                   [[ valid_block xp bn ]]
+    CRASH          MEMLOG.log_intact lxp mbase
+    >} alloc_gen lxp xp mscs.
+  Proof.
+    unfold alloc_gen.
+    intros.
+    eapply pimpl_ok2. apply alloc'_ok.
+    unfold rep_gen, rep'.
+    cancel.
+    step.
+    apply pimpl_or_r. right.
+    norm. (* We can't just [cancel] here because it introduces evars too early *)
+    cancel.
+    intuition.
+
+    pred_apply.
+    cancel.
+
+    assert (a a3 = Avail) as Ha by ( apply H8; eapply remove_still_In; eauto ).
+    rewrite <- Ha.
+    apply fupd_other.
+    eapply remove_still_In_ne; eauto.
+
+    assert (a0 <> a3).
+    intro He. subst. rewrite fupd_same in *. discriminate. trivial.
+    rewrite fupd_other in * by assumption.
+    apply remove_other_In. assumption.
+    rewrite H8; assumption.
+
+    erewrite listpred_remove with (dec := @weq addrlen). cancel.
+    apply ptsto_conflict.
+    rewrite H8; assumption.
+  Qed.
+
+  Theorem free_gen_ok : forall V lxp xp bn mscs,
+    {< Fm mbase m freeblocks genpred,
+    PRE        MEMLOG.rep lxp (ActiveTxn mbase m) mscs *
+               [[ (Fm * @rep_gen V xp freeblocks genpred)%pred (list2mem m) ]] *
+               [[ (bn < BmapNBlocks xp ^* $ valulen)%word ]]
+    POST:mscs' exists m' genpred', MEMLOG.rep lxp (ActiveTxn mbase m') mscs' *
+               [[ (Fm * @rep_gen V xp (bn :: freeblocks) genpred')%pred (list2mem m') ]] *
+               [[ bn |->? * genpred =p=> genpred' ]]
+    CRASH      MEMLOG.log_intact lxp mbase
+    >} free_gen lxp xp bn mscs.
+  Proof.
+    unfold free_gen.
+    intros.
+    eapply pimpl_ok2. apply free'_ok.
+    unfold rep_gen, rep'.
+    cancel.
+    step.
+    subst; apply fupd_same; trivial.
+    rewrite H9 in H3.
+    destruct (weq bn a1).
+    subst; apply fupd_same; trivial.
+    rewrite <- H3; apply fupd_other; assumption.
+    destruct (weq bn a1).
+    left. auto.
+    right. rewrite fupd_other in H0 by assumption. apply H9; assumption.
+  Qed.
+
+  Hint Extern 1 ({{_}} progseq (BALLOC.alloc_gen _ _ _) _) => apply BALLOC.alloc_gen_ok : prog.
+  Hint Extern 1 ({{_}} progseq (BALLOC.free_gen _ _ _ _) _) => apply BALLOC.free_gen_ok : prog.
+  Hint Extern 0 (okToUnify (rep_gen _ _ _) (rep_gen _ _ _)) => constructor : okToUnify.
+
+  (* Different names for actual on-disk-block allocation *)
+  Definition alloc := alloc_gen.
+  Definition free := free_gen.
+
+  Definition rep xp (freeblocks : list addr) :=
+    (exists genpred, genpred * rep_gen xp freeblocks genpred)%pred.
 
   Theorem alloc_ok : forall lxp xp mscs,
     {< Fm mbase m freeblocks,
@@ -217,36 +298,15 @@ Module BALLOC.
     CRASH          MEMLOG.log_intact lxp mbase
     >} alloc lxp xp mscs.
   Proof.
-    unfold alloc.
+    unfold alloc, rep.
     intros.
-    eapply pimpl_ok2. apply alloc'_ok.
-    unfold rep, rep'.
+    eapply pimpl_ok2. apply alloc_gen_ok.
     cancel.
     step.
+    rewrite H9 in H0.
     apply pimpl_or_r. right.
-    norm. (* We can't just [cancel] here because it introduces evars too early *)
     cancel.
-    intuition.
-
-    pred_apply.
-    (* instantiate (a1 := remove (@weq addrlen) a0 l). *)
-    erewrite listpred_remove with (dec := @weq addrlen). cancel.
-    assert (a a3 = Avail) as Ha.
-    apply H8.
-    eapply remove_still_In; eauto.
-    rewrite <- Ha.
-    apply fupd_other.
-    eapply remove_still_In_ne; eauto.
-    assert (a0 <> a3).
-    intro He. subst. rewrite fupd_same in *. discriminate. trivial.
-    rewrite fupd_other in * by assumption.
-    apply remove_other_In. assumption.
-    rewrite H8; assumption.
-    apply ptsto_conflict.
-    rewrite H8; assumption.
   Qed.
-
-
 
   Theorem free_ok : forall lxp xp bn mscs,
     {< Fm mbase m freeblocks,
@@ -258,27 +318,15 @@ Module BALLOC.
     CRASH      MEMLOG.log_intact lxp mbase
     >} free lxp xp bn mscs.
   Proof.
-    unfold free.
+    unfold free, rep.
     intros.
-    eapply pimpl_ok2. apply free'_ok.
-    unfold rep, rep'.
+    eapply pimpl_ok2. apply free_gen_ok.
     cancel.
     step.
-    subst; apply fupd_same; trivial.
-    rewrite H10 in H3.
-    destruct (weq bn a1).
-    subst; apply fupd_same; trivial.
-    rewrite <- H3; apply fupd_other; assumption.
-    destruct (weq bn a1).
-    left. auto.
-    right. rewrite fupd_other in H0 by assumption. apply H10; assumption.
   Qed.
-
-
-  Hint Extern 0 (okToUnify (rep _ _) (rep _ _)) => constructor : okToUnify.
 
   Hint Extern 1 ({{_}} progseq (BALLOC.alloc _ _ _) _) => apply BALLOC.alloc_ok : prog.
   Hint Extern 1 ({{_}} progseq (BALLOC.free _ _ _ _) _) => apply BALLOC.free_ok : prog.
-
+  Hint Extern 0 (okToUnify (rep _ _) (rep _ _)) => constructor : okToUnify.
 
 End BALLOC.
